\let\negmedspace\undefined
\let\negthickspace\undefined
\documentclass[journal]{IEEEtran}
\usepackage[a5paper, margin=10mm, onecolumn]{geometry}
%\usepackage{lmodern} % Ensure lmodern is loaded for pdflatex
\usepackage{tfrupee} % Include tfrupee package

\setlength{\headheight}{1cm} % Set the height of the header box
\setlength{\headsep}{0mm}     % Set the distance between the header box and the top of the text

\usepackage{gvv-book}
\usepackage{gvv}
\usepackage{cite}
\usepackage{amsmath,amssymb,amsfonts,amsthm}
\usepackage{algorithmic}
\usepackage{graphicx}
\usepackage{textcomp}
\usepackage{xcolor}
\usepackage{txfonts}
\usepackage{listings}
\usepackage{enumitem}
\usepackage{mathtools}
\usepackage{gensymb}
\usepackage{comment}
\usepackage[breaklinks=true]{hyperref}
\usepackage{tkz-euclide} 
\usepackage{listings}
% \usepackage{gvv}                                        
\def\inputGnumericTable{}                                 
\usepackage[latin1]{inputenc}                                
\usepackage{color}                                            
\usepackage{array}                                            
\usepackage{longtable}                                       
\usepackage{calc}                                             
\usepackage{multirow}                                         
\usepackage{hhline}                                           
\usepackage{ifthen}                                           
\usepackage{lscape}
\usepackage{multicol}
\begin{document}

\bibliographystyle{IEEEtran}
\vspace{3cm}

\title{5.13.38}
\author{EE25BTECH11012-BEERAM MADHURI}
% \maketitle
% \newpage
% \bigskip
{\let\newpage\relax\maketitle}

\renewcommand{\thefigure}{\theenumi}
\renewcommand{\thetable}{\theenumi}
\setlength{\intextsep}{10pt} % Space between text and floats


\numberwithin{equation}{enumi}
\numberwithin{figure}{enumi}
\renewcommand{\thetable}{\theenumi}


\textbf{Question}:\\
Let $\mathbf{X}$ and $\mathbf{Y}$ be two arbitrary, $3 \times 3$, non-zero, skew-symmetric matrices and $\mathbf{Z}$ be an arbitrary $3 \times 3$, non-zero, symmetric matrix. Then which of the following matrices is (are) skew symmetric?

\begin{enumerate}
\begin{multicols}{4}
    \item $\mathbf{Y}^3 \mathbf{Z}^4 - \mathbf{Z}^4 \mathbf{Y}^3$
    \item $\mathbf{X}^{44} + \mathbf{Y}^{44}$
    \item $\mathbf{X}^4 \mathbf{Z}^3 - \mathbf{Z}^3 \mathbf{X}^4$
    \item $\mathbf{X}^{23} + \mathbf{Y}^{23}$
\end{multicols}
\end{enumerate}

\textbf{Solution:}\\
Given,
\begin{align}
\begin{aligned}\vec{X}^\top &= -\vec{X} \quad (\text{Skew-Symmetric}) \\\vec{Y}^\top &= -\vec{Y} \quad (\text{Skew-Symmetric}) \\\vec{Z^\top} &= \vec{Z} \quad (\text{Symmetric})\end{aligned}
\end{align}
Checking all options:\\
a) $\vec{Y^3 Z^4} - \vec{Z^4 Y^3}$\\
Let 
\begin{align}
A = \vec{Y^3 Z^4} - \vec{Z^4 Y^3}\\
A^\top &= (\vec{Y^3 Z^4} - \vec{Z^4 Y^3})^\top \\
A^\top &= (\vec{Y^3 Z^4})^\top - (\vec{Z^4 Y^3})^\top \\
A^\top &= (\vec{Z}^\top)^4 (\vec{Y}^\top)^3 - (\vec{Y}^\top)^3 (\vec{Z}^\top)^4 \\
A^\top &= (\vec{Z}^\top)^4 (\vec{Y}^\top)^3 - (\vec{Y}^\top)^3 (\vec{Z}^\top)^4\end{align}

Now, substitute the given properties ($\vec{Z}^\top= \vec{Z}$ and $\vec{Y}^\top = -\vec{Y}$):
\begin{align}A^\top &= (\vec{Z})^4 (-\vec{Y})^3 - (-\vec{Y})^3 (\vec{Z})^4 \\
\text{Since } (-\vec{Y})^3 &= (-1)^3 \vec{Y}^3 = -\vec{Y}^3, \text{ we get:} \\
A^\top &= \vec{Z}^4 (-\vec{Y}^3) - (-\vec{Y}^3) \vec{Z}^4 \\
A^\top &= -\vec{Z}^4 \vec{Y}^3 + \vec{Y}^3 \vec{Z}^4 \\
A^\top &= \vec{Y}^3 \vec{Z}^4 - \vec{Z}^4 \vec{Y}^3\\
=\vec{A}\end{align}
Hence, $A$ is Symmetric Matrix.\\

b) $\vec{X}^{44} + \vec{Y}^{44}$\\
Let 
\begin{align}
B = \vec{X}^{44} + \vec{Y}^{44}\\
B^\top = (\vec{X}^{44} + \vec{Y}^{44})^\top \\
B^\top = (\vec{X}^{44})^\top + (\vec{Y}^{44})^\top \\
B^\top = (\vec{X}^\top)^{44} + (\vec{Y}^\top)^{44}
\end{align}

Now, substitute the given properties ($\vec{X}^\top = -\vec{X}$ and $\vec{Y}^\top = -\vec{Y}$):
\begin{align}
B^\top = (-\vec{X})^{44} + (-\vec{Y})^{44}\\
(-1)^{44} = 1 \\
\therefore (-\vec{X})^{44} = \vec{X}^{44} and (-\vec{Y})^{44} = \vec{Y}^{44} \\
B^\top = \vec{X}^{44} + \vec{Y}^{44}\\
B^\top=B
\end{align}
Hence, $B$ is Symmetric Matrix.\\

c)  $\vec{X}^4\vec{Z}^3 - \vec{Z}^3\vec{X}^4$\\Let
\begin{align}
C&=(\vec{X^4Z^3} - \vec{Z^3X^4})\\
C^\top &= (\vec{X^4Z^3} - \vec{Z^3X^4})^\top \\
C^\top &= (\vec{X^4Z^3})^\top - (\vec{Z^3X^4})^\top \\
C^\top &= (\vec{Z}^3)^\top(\vec{X}^4)^\top - (\vec{X}^4)^\top(\vec{Z}^3)^\top \\
C^\top &= (\vec{Z}^\top)^3(\vec{X}^\top)^4 - (\vec{X}^\top)^4(\vec{Z}^\top)^3
\end{align}

Now, substitute the given properties ($\vec{Z}^\top = \vec{Z}$ and $\vec{X}^\top = -\vec{X}$):
\begin{align}
C^\top&= (\vec{Z})^3(-\vec{X})^4 - (-\vec{X})^4(\vec{Z})^3 \\
(-\vec{X})^4 &= \vec{X}^4 \\
\vec{C}^\top &= \vec{Z}^3\vec{X}^4 - \vec{X}^4\vec{Z}^3 \\
C^\top &= -(\vec{X}^4\vec{Z}^3 - \vec{Z}^3\vec{X}^4)\\
=-C
\end{align}
Hence, $C$ is Skew Symmetric Matrix.\\

d) $\vec{X^{23} + Y}^{23}$\\Let
\begin{align}
D&=\vec{X}^{23} + \vec{Y}^{23}\\
D^\top &= (\vec{X}^{23} + \vec{Y}^{23})^\top \\
D^\top &= (\vec{X}^{23})^\top + (\vec{Y}^{23})^\top \\
D^\top &= (\vec{X}^\top)^{23} + (\vec{Y}^\top)^{23}
\end{align}
Now, substitute the given properties ($\vec{X}^\top = -\vec{X}$ and $\vec{Y}^\top = -\vec{Y}$):
\begin{align}
D^\top &= (-\vec{X})^{23} + (-\vec{Y})^{23} \\
(-1)^{23} = -1\\
(-\vec{X})^{23} = -\vec{X}^{23} \text{ and } (-\vec{Y})^{23} = -\vec{Y}^{23}\\
D^\top &= -\vec{X}^{23} - \vec{Y}^{23} \\
D^\top &= -(\vec{X}^{23} + \vec{Y}^{23})\\
=-D
\end{align}
Hence, $D$ is Skew Symmetric Matrix.\\\\
$\therefore$ Option 3. $\vec{X}^4\vec{Z}^3 - \vec{Z}^3\vec{X}^4$ and\\ 
Option 4. $\vec{X^{23} + Y}^{23}$ are Skew Symmetric
\end{document}