\documentclass[a4paper, 12pt]{article}

\usepackage{geometry}
\usepackage{amsmath}
\usepackage{gvv}

\title{Question 5.13.26}
\author{AI25BTECH11040 - Vivaan Parashar}
\date{\today}

\begin{document}

\maketitle

\section{Question: }
If $\vec{A}$ and $\vec{B}$ are square matrices of size $n \times n$ such that $\vec{A}^2 - \vec{B}^2 = (\vec{A} - \vec{B}) (\vec{A} + \vec{B})$, then which of the following will be always true?
\begin{enumerate}[label=(\alph*)]
    \item $\vec{A} = \vec{B}$
    \item $\vec{AB} = \vec{BA}$
    \item either of $\vec{A}$ or $\vec{B}$ is a zero matrix
    \item either $\vec{A}$ or $\vec{B}$ is an identity matrix
\end{enumerate}

\section{Solution: }
We know that for any two square matrices $\vec{A}$ and $\vec{B}$ of size $n \times n$, the following is true:
\begin{align}
    (\vec{A} - \vec{B}) (\vec{A} + \vec{B}) &= (\vec{A} - \vec{B})\vec{A} + (\vec{A} - \vec{B})\vec{B}\\
    &= \vec{A}^2 - \vec{BA} + \vec{AB} - \vec{B}^2 \label{eq1}
\end{align}
Given that $\vec{A}^2 - \vec{B}^2 = (\vec{A} - \vec{B}) (\vec{A} + \vec{B})$, we can use equation \ref{eq1}:
\begin{align}
    \vec{A}^2 - \vec{B}^2 &= \vec{A}^2 - \vec{BA} + \vec{AB} - \vec{B}^2\\
    \implies 0 &= - \vec{BA} + \vec{AB}\\
    \implies \vec{BA} &= \vec{AB}
\end{align}
Thus, option (b) is always true.

\end{document}