\documentclass[12pt]{article}
\usepackage{graphicx}
\usepackage{enumitem}
\usepackage{amsmath}
\usepackage{gvv-book}
\usepackage{gvv}

\title{\textbf{5.13.34}}
\author{\textbf{EE25BTECH11008 - Anirudh M Abhilash}}
\date{October 5, 2025}

\begin{document}

\maketitle

\section*{Question}

For $3 \times 3$ matrices $\vec{M}$ and $\vec{N}$, which of the following statement(s) is (are) \textbf{NOT} correct?  

\begin{multicols}{2}
\begin{enumerate}[label=(\alph*)]
\item $\vec{N}^T \vec{M} \vec{N}$ is symmetric or skew symmetric, according as $\vec{M}$ is symmetric or skew symmetric.
\item $\vec{M}\vec{N} - \vec{N}\vec{M}$ is skew symmetric for all matrices $\vec{M}$ and $\vec{N}$.
\item $\vec{M}\vec{N}$ is symmetric for all symmetric matrices $\vec{M}$ and $\vec{N}$.
\item $(\operatorname{adj}\vec{M})(\operatorname{adj}\vec{N}) = \operatorname{adj}(\vec{M}\vec{N})$ for all invertible matrices $\vec{M}$ and $\vec{N}$.
\end{enumerate}
\end{multicols}


\section*{Solution}

\subsection*{(a)}

\begin{align}
(\vec{N}^T \vec{M} \vec{N})^T &= \vec{N}^T \vec{M}^T \vec{N}
\end{align}

If $\vec{M}^T = \vec{M}$,  
\begin{align}
(\vec{N}^T \vec{M} \vec{N})^T = \vec{N}^T \vec{M} \vec{N}
\end{align}
Hence symmetric.

If $\vec{M}^T = -\vec{M}$,  
\begin{align}
(\vec{N}^T \vec{M} \vec{N})^T = -\vec{N}^T \vec{M} \vec{N}
\end{align}
Hence skew symmetric.  

Thus, (a) is \textbf{correct}.

\subsection*{(b)}

Assume $\vec{M}\vec{N} - \vec{N}\vec{M}$ is skew symmetric $\forall \, \vec{M}, \vec{N}$.

Then,
\begin{align}
(\vec{M}\vec{N} - \vec{N}\vec{M})^T &= -(\vec{M}\vec{N} - \vec{N}\vec{M}) \\
\Rightarrow \vec{N}^T \vec{M}^T - \vec{M}^T \vec{N}^T &= -\vec{M}\vec{N} + \vec{N}\vec{M}
\end{align}

Let $\vec{M}$ and $\vec{N}$ be symmetric:
\begin{align}
\vec{M}^T = \vec{M}, \quad \vec{N}^T = \vec{N}
\end{align}
Then,
\begin{align}
\vec{N}\vec{M} - \vec{M}\vec{N} &= -\vec{M}\vec{N} + \vec{N}\vec{M} \\
\Rightarrow 2(\vec{N}\vec{M} - \vec{M}\vec{N}) &= 0 \\
\Rightarrow \vec{M}\vec{N} = \vec{N}\vec{M}
\end{align}

Thus, this requires all symmetric matrices to commute, which is not true in general.  
Hence, (b) is \textbf{not correct}.

\subsection*{(c)}

\begin{align}
(\vec{M}\vec{N})^T &= \vec{N}^T \vec{M}^T
\end{align}

If $\vec{M}$ and $\vec{N}$ are symmetric,
\begin{align}
(\vec{M}\vec{N})^T &= \vec{N}\vec{M}
\end{align}
For $\vec{M}\vec{N}$ to be symmetric,  
\begin{align}
\vec{M}\vec{N} &= \vec{N}\vec{M}
\end{align}
Thus, $\vec{M}\vec{N}$ is symmetric $\iff$ $\vec{M}$ and $\vec{N}$ commute.  
Since all symmetric matrices do not commute, (c) is \textbf{not correct}.

\subsection*{(d)}

For any invertible matrix $\vec{A}$,
\begin{align}
\operatorname{adj}(\vec{A}) = \mydet{\vec{A}} \vec{A}^{-1}
\end{align}

Hence,
\begin{align}
(\operatorname{adj}\vec{M})(\operatorname{adj}\vec{N}) &= \mydet{\vec{M}}\mydet{\vec{N}}\vec{M}^{-1}\vec{N}^{-1}, \\[4pt]
\operatorname{adj}(\vec{M}\vec{N}) &= \mydet{\vec{M}\vec{N}}(\vec{M}\vec{N})^{-1} = \mydet{\vec{M}}\mydet{\vec{N}} \vec{N}^{-1}\vec{M}^{-1}.
\end{align}

Equality holds only if  
\begin{align}
\vec{M}^{-1}\vec{N}^{-1} = \vec{N}^{-1}\vec{M}^{-1} \iff \vec{M}\vec{N} = \vec{N}\vec{M}.
\end{align}

Since this does not hold for all invertible matrices, (d) is \textbf{not correct}.

\[
\boxed{\text{Statements (b), (c), and (d) are NOT correct.}}
\]

\end{document}
