\documentclass{beamer}
\usepackage{amsmath}
\usepackage{gvv}

\newcommand\numberthis{\addtocounter{equation}{1}\tag{\theequation}}

\title{Question 4.2.3}
\author{AI25BTECH11040 - Vivaan Parashar}
\date{\today}

\begin{document}

\frame{\titlepage}

\begin{frame}
    \frametitle{Question: }
    Given $\vec{A} = \myvec{2 & -3 \\ -4 & 7}$, compute $\vec{A}^{-1}$ and show that $2\vec{A}^{-1} = 9\vec{I} - \vec{A}$.
\end{frame}

\begin{frame}
    \frametitle{Solution: }
    We start by finding the characteristic equation of $\vec{A}$.
    \begin{align*}
        f(\lambda)          & = \det(\vec{A} - \lambda \vec{I})                                       \\
                            & = \det\myvec{\lambda - 2                                            & 3 \\ 4 & \lambda - 7} \\
                            & = (\lambda - 2)(\lambda - 7) - 12                                       \\
                            & = \lambda^2 - 9\lambda + 2                                              \\
        \implies f(\lambda) & = (\lambda - 1)(\lambda - 8) = \lambda^2 - 9\lambda + 2 \numberthis
    \end{align*}
    If we were to set $\lambda = 0$, we get $\det(\vec{A}) = 2 \ne 0$. Thus, $\vec{A}$ is invertible and $\vec{A}^{-1}$ exists. To find it, we use the Cayley-Hamilton theorem that states that the characteristic equation $f(\lambda) = 0$ is also satisfied by the matrix itself, i.e, $f(\vec{A}) = 0$. Thus,
\end{frame}
\begin{frame}
    \begin{align*}
        f(\vec{A})                    & = \vec{A}^2 - 9\vec{A} + 2\vec{I} = 0                        \\
        \implies 2\vec{I}             & = 9\vec{A} - \vec{A}^2                                       \\
        \implies 2\vec{I}\vec{A}^{-1} & = 9\vec{A}\vec{A}^{-1} - \vec{A}^2\vec{A}^{-1}               \\
        \implies 2\vec{A}^{-1}        & = 9\vec{I} - \vec{A}       \numberthis                       \\
        \implies \vec{A}^{-1}         & = \frac{1}{2}\myvec{9 - 2                      & 3           \\ 4 & 9 - 7} \\
        \implies \vec{A}^{-1}         & = \myvec{\frac{7}{2}                           & \frac{3}{2} \\ 2 & 1} \numberthis
    \end{align*}
    Thus, we have computed $\vec{A}^{-1}$ and shown that $2\vec{A}^{-1} = 9\vec{I} - \vec{A}$.
\end{frame}
\end{document}
